1) renamed llvm_op/ssa_static|dynamic.* into llvm_op/ssa_verifier/interpreter.*. Actually what these files defined are not the semantics of SSA, but validator and interpreters that are defined in LLVM. The monads we defined can be taken a DSL to define imperative applications. We should prove that they are sound w.r.t. the semantics.
2) deleted vmcore.v and reflect.v, which were merged into ssa_coq_lib.v

3) added ssa_static.ott, which defines the well-formedness, and tries to
define invariants of SSA. Questions:
   a) The definition of SSA seems obvious informally, but formal
definitions (properties and invariants) are not obvious, did not find
such definitions yet.
   b) also fixed some bugs in ssa_verifier.v.
   c) deleted 'invoke', its semantics has no counterpart in CompCert
   d) the current subset does not have memory operations, which makes
the subset too simple. Adding memory operations also requires to define a
memory model for LLVM.



git-svn-id: https://webdav.seas.upenn.edu/svn/sol/vol@2461 eef5ea85-cc2e-0410-bd84-0fae1f012da8

src/ssa/ssa_coq_lib.v
@@ -139,7 +139,7 @@ Require Import Omega.
   | insn_br t v l1 l2 => None
   | insn_br_uncond l => None
   (* | insn_switch t v l _ => None *)
-  | insn_invoke id typ id0 paraml l1 l2 => Some id
+  (* | insn_invoke id typ id0 paraml l1 l2 => Some id *)
   | insn_call id typ id0 paraml => Some id
   | insn_unreachable => None
   | insn_add id typ v1 v2 => Some id
@@ -212,7 +212,7 @@ Require Import Omega.
   | insn_br t v l1 l2 => genInsnUseDef_value v i b f m        
   | insn_br_uncond l => fun _ => nil
   (* | insn_switch t v l _ => genInsnUseDef_value v i b f m *)
-  | insn_invoke id typ id0 paraml l1 l2 => (genInsnUseDef_id id0 i b f m)+++(genInsnUseDef_params paraml i b f m)
+  (* | insn_invoke id typ id0 paraml l1 l2 => (genInsnUseDef_id id0 i b f m)+++(genInsnUseDef_params paraml i b f m) *)
   | insn_call id typ id0 paraml => fun _ => nil
   | insn_unreachable => fun _ => nil
   | insn_add id typ v1 v2 => (genInsnUseDef_value v1 i b f m)+++(genInsnUseDef_value v2 i b f m)
@@ -321,7 +321,7 @@ Require Import Omega.
   | insn_br t v l1 l2 => genBlockUseDef_label l1 i b f m ++++ genBlockUseDef_label l2 i b f m       
   | insn_br_uncond l => genBlockUseDef_label l i b f m
   (* | insn_switch t v l ls => genBlockUseDef_label l i b f m ++++ genBlockUseDef_switch_cases ls i b f m *)
-  | insn_invoke id typ id0 paraml l1 l2 => (genBlockUseDef_label l1 i b f m)++++(genBlockUseDef_label l2 i b f m)
+  (* | insn_invoke id typ id0 paraml l1 l2 => (genBlockUseDef_label l1 i b f m)++++(genBlockUseDef_label l2 i b f m) *)
   | insn_call id typ id0 paraml => fun _ => nil
   | insn_unreachable => fun _ => nil 
   | insn_add id typ v1 v2 => fun _ => nil 
@@ -412,7 +412,7 @@ Require Import Omega.
   | insn_br t v l1 l2 => lset_add l1 (lset_add l2 lempty_set)
   | insn_br_uncond l0 => lset_add l0 lempty_set 
   (* | insn_switch t v l0 cls => lset_add l0 (getLabelsFromSwitchCases cls) *)
-  | insn_invoke id typ id0 ps l1 l2 => lset_add l1 (lset_add l2 lempty_set)
+  (* | insn_invoke id typ id0 ps l1 l2 => lset_add l1 (lset_add l2 lempty_set) *)
   | _ => empty_set l
   end.
 
@@ -632,11 +632,13 @@ match t with
 | _ => false
 end.
 
+(*
 Definition isInvokeInsnB (i:insn) : bool :=
 match i with
 | insn_invoke _ _ _ _ _ _ => true
 | _ => false
 end.
+*)
 
 Definition isReturnInsnB (i:insn) : bool :=
 match i with
@@ -703,7 +705,7 @@ match i with
 | insn_br _ _ _ _ => true
 | insn_br_uncond _ => true
 (* | insn_switch _ _ _ => true *)
-| insn_invoke _ _ _ _ _ _ => true
+(* | insn_invoke _ _ _ _ _ _ => true *)
 | insn_call _ _ _ _ => true
 | insn_unreachable => true
 | _ => false
@@ -737,7 +739,7 @@ match i with
 | insn_br typ _ _ _ => None 
 | insn_br_uncond _ => None
 (* | insn_switch typ _ _ _ => None *)
-| insn_invoke _ typ _ _ _ _ => Some typ
+(* | insn_invoke _ typ _ _ _ _ => Some typ *)
 | insn_call _ typ _ _ => Some typ
 | insn_unreachable => None
 | insn_add _ typ _ _ => Some typ
@@ -804,7 +806,7 @@ match i with
 | insn_br _ v _ _ => getValueIDsC v
 | insn_br_uncond _ => nil
 (* | insn_switch _ value _ _ => getValueIDs value *)
-| insn_invoke _ _ _ lp _ _ => getParamsOperandC lp
+(* | insn_invoke _ _ _ lp _ _ => getParamsOperandC lp *)
 | insn_call _ _ _ lp => getParamsOperandC lp
 | insn_unreachable => nil
 | insn_add _ _ v1 v2 => getValueIDsC v1 ++ getValueIDsC v2
@@ -841,7 +843,7 @@ match i with
 | insn_br _ _ l1 l2 => l1::l2::nil
 | insn_br_uncond l => l::nil
 (* | insn_switch _ _ l ls => l::list_prj2 _ _ ls *)
-| insn_invoke _ _ _ _ l1 l2 => l1::l2::nil
+(* | insn_invoke _ _ _ _ l1 l2 => l1::l2::nil *)
 | insn_call _ _ _ _ => nil
 | insn_unreachable => nil
 | insn_add _ _ _ _ => nil
@@ -948,6 +950,7 @@ match fd with
 | fdef_intro fh _ => getFheaderIDC fh
 end.
 
+(*
 Definition getNormalDestFromInvokeInsnC (i:insn) : option l :=
 match i with
 | insn_invoke _ _ _ _ l1 _ => Some l1
@@ -959,6 +962,7 @@ match i with
 | insn_invoke _ _ _ _ _ l2 => Some l2
 | _ => None
 end.
+*)
 
 Fixpoint getLabelViaIDFromList (ls:list (id*l)) (branch:id) : option l :=
 match ls with
@@ -1479,6 +1483,7 @@ match (i, i') with
   beq_nat l1 l1' && beq_nat l2 l2'
 | (insn_br_uncond l, insn_br_uncond l') =>
   beq_nat l l'
+(*
 | (insn_invoke id typ id0 paraml l1 l2,
    insn_invoke id' typ' id0' paraml' l1' l2') =>
   beq_nat id id' &&
@@ -1487,6 +1492,7 @@ match (i, i') with
   list_param_EqB paraml paraml' &&
   beq_nat l1 l1' &&
   beq_nat l2 l2'
+*)
 | (insn_call id typ id0 paraml,
    insn_call id' typ' id0' paraml') =>
   beq_nat id id' &&
@@ -1741,6 +1747,467 @@ Notation "t =t= t' " := (typEqB t t') (at level 50).
 Notation "n =n= n'" := (beq_nat n n') (at level 50).
 Notation "b =b= b'" := (blockEqB b b') (at level 50).
 Notation "i =i= i'" := (insnEqB i i') (at level 50).
+
+(**********************************)
+(* Check to make sure that if there is more than one entry for a
+   particular basic block in this PHI node, that the incoming values 
+   are all identical. *)
+Fixpoint lookupIdsViaLabelFromIdls (idls:list (id*l)) (l0:l) : list id :=
+match idls with
+| nil => nil
+| (id1,l1)::idls' =>
+  if (beq_nat l0 l1) 
+  then set_add eq_nat_dec id1 (lookupIdsViaLabelFromIdls idls' l0)
+  else (lookupIdsViaLabelFromIdls idls' l0)
+end.
+
+Fixpoint _checkIdenticalIncomingValues (idls idls0:list (id*l)) : Prop :=
+match idls with
+| nil => True
+| (id, l)::idls' => 
+  (length (lookupIdsViaLabelFromIdls idls0 l) <= 1) /\
+  (_checkIdenticalIncomingValues idls' idls0)
+end.
+
+Definition checkIdenticalIncomingValues (PN:insn) : Prop :=
+match PN with
+| insn_phi _ _ idls => _checkIdenticalIncomingValues idls idls
+| _ => False
+end.
+
+(**********************************)
+(* Instruction Signature *)
+
+Module Type SigValue.
+
+ Parameter getNumOperands : insn -> nat.
+
+End SigValue.
+
+Module Type SigUser. 
+ Include Type SigValue.
+
+End SigUser.
+
+Module Type SigConstant.
+ Include Type SigValue.
+
+End SigConstant.
+
+Module Type SigGlobalValue.
+ Include Type SigConstant.
+
+End SigGlobalValue.
+
+Module Type SigFunction.
+ Include Type SigGlobalValue.
+
+ Parameter getDefReturnType : fdef -> typ.
+ Parameter getDefFunctionType : fdef -> typ.
+ Parameter def_arg_size : fdef -> nat.
+ 
+ Parameter getDecReturnType : fdec -> typ.
+ Parameter getDecFunctionType : fdec -> typ.
+ Parameter dec_arg_size : fdec -> nat.
+
+End SigFunction.
+
+Module Type SigInstruction.
+ Include Type SigUser.
+
+(* Parameter isInvokeInst : insn -> bool. *)
+ Parameter isCallInst : insn -> bool.
+
+End SigInstruction.
+
+Module Type SigReturnInst.
+ Include Type SigInstruction.
+
+ Parameter hasReturnType : insn -> bool.
+ Parameter getReturnType : insn -> option typ.
+
+End SigReturnInst.
+
+Module Type SigCallSite.
+ Parameter getCalledFunction : insn -> system -> option fdef.
+ Parameter getFdefTyp : fdef -> typ.
+ Parameter arg_size : fdef -> nat.
+ Parameter getArgument : fdef -> nat -> option arg.
+ Parameter getArgumentType : fdef -> nat -> option typ.
+
+End SigCallSite.
+
+Module Type SigCallInst.
+ Include Type SigInstruction.
+
+End SigCallInst.
+
+(*
+Module Type SigInvokeInst.
+ Include Type SigInstruction.
+
+ Parameter getNormalDest : system -> insn -> option block.
+
+End SigInvokeInst.
+*)
+
+Module Type SigBinaryOperator.
+ Include Type SigInstruction.
+
+ Parameter getFirstOperandType : system -> insn -> option typ.
+ Parameter getSecondOperandType : system -> insn -> option typ.
+ Parameter getResultType : insn -> option typ.
+
+End SigBinaryOperator.
+
+Module Type SigPHINode.
+ Include Type SigInstruction.
+
+ Parameter getNumIncomingValues : insn -> option nat.
+ Parameter getIncomingValueType : system  -> insn -> i -> option typ.
+End SigPHINode.
+
+(* Type Signature *)
+
+Module Type SigType.
+ Parameter isIntOrIntVector : typ -> bool.
+ Parameter isInteger : typ -> bool.
+End SigType.
+
+Module Type SigDerivedType.
+ Include Type SigType.
+End SigDerivedType.
+
+Module Type SigFunctionType.
+ Include Type SigDerivedType.
+
+ Parameter getNumParams : typ -> option nat.
+ Parameter isVarArg : typ -> bool.
+ Parameter getParamType : typ -> nat -> option typ.
+End SigFunctionType.
+
+Module Type SigCompositeType.
+ Include Type SigDerivedType.
+End SigCompositeType.
+
+Module Type SigSequentialType.
+ Include Type SigCompositeType.
+
+ Parameter hasElementType : typ -> bool.
+ Parameter getElementType : typ -> option typ.
+
+End SigSequentialType.
+
+Module Type SigArrayType.
+ Include Type SigSequentialType.
+
+ Parameter getNumElements : typ -> nat.
+
+End SigArrayType.
+
+(* Instruction Instantiation *)
+
+Module Value <: SigValue.
+
+ Definition getNumOperands (i:insn) : nat := 
+   length (getInsnOperandsC i).  
+
+End Value.
+
+Module User <: SigUser. Include Value.
+
+End User.
+
+Module Constant <: SigConstant.
+ Include Value.
+
+End Constant.
+
+Module GlobalValue <: SigGlobalValue.
+ Include Constant.
+
+End GlobalValue.
+
+Module Function <: SigFunction.
+ Include GlobalValue.
+
+ Definition getDefReturnType (fd:fdef) : typ :=
+ match fd with
+ | fdef_intro (fheader_intro t _ _) _ => t
+ end.
+
+ Definition getDefFunctionType (fd:fdef) : typ := getFdefTypC fd.
+
+ Definition def_arg_size (fd:fdef) : nat :=
+ match fd with
+ | (fdef_intro (fheader_intro _ _ la) _) => length la
+ end.
+
+ Definition getDecReturnType (fd:fdec) : typ :=
+ match fd with
+ | fdec_intro (fheader_intro t _ _) => t
+ end.
+
+ Definition getDecFunctionType (fd:fdec) : typ := getFdecTypC fd.
+
+ Definition dec_arg_size (fd:fdec) : nat :=
+ match fd with
+ | (fdec_intro (fheader_intro _ _ la)) => length la
+ end.
+
+End Function.
+
+Module Instruction <: SigInstruction.
+ Include User.
+
+(* Definition isInvokeInst (i:insn) : bool := isInvokeInsnB i. *)
+ Definition isCallInst (i:insn) : bool := isCallInsnB i.
+
+End Instruction.
+
+Module ReturnInst <: SigReturnInst.
+ Include Instruction.
+
+ Definition hasReturnType (i:insn) : bool :=
+ match i with
+ | insn_return t v => true
+ | _ => false
+ end.
+
+ Definition getReturnType (i:insn) : option typ :=
+ match i with
+ | insn_return t v => Some t
+ | _ => None
+ end.
+
+End ReturnInst.
+
+Module CallSite <: SigCallSite.
+
+ Definition getCalledFunction (i:insn) (s:system) : option fdef :=
+ match i with 
+ (* | insn_invoke _ _ fid _ _ _ => lookupFdefViaIDFromSystemC s fid *)
+ | insn_call _ _ fid _ => lookupFdefViaIDFromSystemC s fid
+ | _ => None
+ end.
+
+ Definition getFdefTyp (fd:fdef) : typ := getFdefTypC fd.
+
+ Definition arg_size (fd:fdef) : nat :=
+ match fd with
+ | (fdef_intro (fheader_intro _ _ la) _) => length la
+ end.
+
+ Definition getArgument (fd:fdef) (i:nat) : option arg :=
+ match fd with
+ | (fdef_intro (fheader_intro _ _ la) _) => 
+    match (nth_error la i) with
+    | Some a => Some a
+    | None => None
+    end
+ end. 
+
+ Definition getArgumentType (fd:fdef) (i:nat) : option typ :=
+ match (getArgument fd i) with
+ | Some (t, _) => Some t
+ | None => None
+ end.
+
+End CallSite.
+
+Module CallInst <: SigCallInst.
+ Include Instruction.
+
+End CallInst.
+
+(*
+Module InvokeInst <: SigInvokeInst.
+ Include Instruction.
+
+ Definition getNormalDest (s:system) (i:insn) : option block :=
+ match (getNormalDestFromInvokeInsnC i) with
+ | None => None
+ | Some l => lookupBlockViaLabelFromSystem s l
+ end.
+
+End InvokeInst.
+*)
+
+Module BinaryOperator <: SigBinaryOperator.
+ Include Instruction.
+
+ Definition getFirstOperandType (s:system) (i:insn) : option typ := 
+ match i with
+ | insn_add _ _ v1 _ => 
+   match v1 with
+   | value_id id1 => lookupTypViaIDFromSystemC s id1
+   | _ => Some (typ_int 0) (* FIXME: how to set the type of const*)
+   end
+ | _ => None
+ end.
+
+ Definition getSecondOperandType (s:system) (i:insn) : option typ := 
+ match i with
+ | insn_add _ _ _ v2 => 
+   match v2 with
+   | value_id id2 => lookupTypViaIDFromSystemC s id2
+   | _ => Some (typ_int 0) (* FIXME: how to set the type of const*)
+   end
+ | _ => None
+ end.
+
+ Definition getResultType (i:insn) : option typ := getInsnTypC i.
+
+End BinaryOperator.
+
+Module PHINode <: SigPHINode.
+ Include Instruction.
+
+ Definition getNumIncomingValues (i:insn) : option nat :=
+ match i with
+ | (insn_phi _ _ ln) => Some (length ln)
+ | _ => None
+ end.
+
+ Definition getIncomingValueType (s:system) (i:insn) (n:nat) : option typ :=
+ match i with
+ | (insn_phi _ _ ln) => 
+    match (nth_error ln n) with
+    | Some (id, _) => lookupTypViaIDFromSystemC s id
+    | None => None
+    end
+ | _ => None
+ end.
+
+End PHINode.
+
+(* Type Instantiation *)
+
+Module Typ <: SigType.
+ Definition isIntOrIntVector (t:typ) : bool :=
+ match t with
+ | typ_int _ => true
+ | _ => false
+ end.
+
+ Definition isInteger (t:typ) : bool :=
+ match t with
+ | typ_int _ => true
+ | _ => false
+ end.
+
+End Typ.
+
+Module DerivedType <: SigDerivedType.
+ Include Typ.
+End DerivedType.
+
+Module FunctionType <: SigFunctionType.
+ Include DerivedType.
+
+ Definition getNumParams (t:typ) : option nat :=
+ match t with
+ | (typ_function _ lt) => Some (length lt)
+ | _ => None
+ end.
+
+ Definition isVarArg (t:typ) : bool := false.
+
+ Definition getParamType (t:typ) (i:nat) : option typ :=
+ match t with
+ | (typ_function _ lt) => 
+    match (nth_error lt i) with
+    | Some t => Some t
+    | None => None
+    end
+ | _ => None
+ end.
+
+End FunctionType.
+
+Module CompositeType <: SigCompositeType.
+ Include DerivedType.
+End CompositeType.
+
+Module SequentialType <: SigSequentialType.
+ Include CompositeType.
+
+ Definition hasElementType (t:typ) : bool :=
+ match t with
+ | typ_array _ t' => true
+ | _ => false
+ end.
+
+ Definition getElementType (t:typ) : option typ :=
+ match t with
+ | typ_array _ t' => Some t'
+ | _ => None
+ end.
+
+End SequentialType.
+
+Module ArrayType <: SigArrayType.
+ Include SequentialType.
+
+ Definition getNumElements (t:typ) : nat :=
+ match t with
+ | typ_array N _ => N
+ | _ => 0
+ end.
+
+End ArrayType.
+
+(**********************************)
+(* reflect *)
+
+Require Import Decidable.
+
+Section Decidable.
+
+Lemma dec_blockDominates : forall (d:dt) (b1 b2: block),
+  decidable (blockDominates d b1 b2).
+Proof.
+  intros d b1 b2.
+  unfold decidable. unfold blockDominates.
+  destruct b1 as [l1 insns1].
+  destruct b2 as [l2 insns2].
+  remember (lset_mem l2 (d l1)) as c.
+  destruct c; auto.
+Qed.
+
+End Decidable.
+
+Coercion is_true (b:bool) := b = true.
+
+Inductive reflect (P:Prop) : bool -> Set :=
+| ReflectT : P -> reflect P true
+| ReflectF : ~P -> reflect P false
+.
+
+Section Reflect.
+
+Lemma reflect_blockDominates : forall d b1 b2,
+  reflect (blockDominates d b1 b2) (blockDominatesB d b1 b2).
+Proof.
+  intros d b1 b2.
+  unfold blockDominates. unfold blockDominatesB.
+  destruct b1 as [l1 insns1].
+  destruct b2 as [l2 insns2].
+  remember (lset_mem l2 (d l1)) as c.
+  destruct c; auto.
+    apply ReflectT; auto.
+    apply ReflectF; auto.
+Qed.
+
+Require Import monad.
+
+Definition ifP d b1 b2 (X:Type) (t f : monad X) :=
+match (reflect_blockDominates d b1 b2) with
+| ReflectT _ => t
+| ReflectF _ => f
+end.
+
+End Reflect.
 
 (*ENDCOPY*)
 
